theories/base_logic/gen_sim_prog.v
@@ -7,19 +7,19 @@ From iris.prelude Require Import options.
   It provides a persistent token f @ K asserting that there is a function f with body K.
 *)
 
-Class gen_progPreG (F C : Type) (Σ : gFunctors) `{Countable F} := {
+Class gen_progGpreS (F C : Type) (Σ : gFunctors) `{Countable F} := {
   gen_prog_preG_inG :> ghost_mapG Σ F C;
 }.
 
-Class gen_progPreNameG (F C : Type) (Σ : gFunctors) (gen_prog_name : gname) `{Countable F} := GenProgPreNameG {
-  gen_prog_preNameG :> gen_progPreG F C Σ
+Class gen_progGS_named (F C : Type) (Σ : gFunctors) (gen_prog_name : gname) `{Countable F} := GenProgGSNamed {
+  gen_prog_preNameG :> gen_progGpreS F C Σ
 }.
 
-Class gen_sim_progG (F C_t C_s : Type) (Σ : gFunctors) `{Countable F} := GenSimProgG {
+Class gen_sim_progGS (F C_t C_s : Type) (Σ : gFunctors) `{Countable F} := GenSimProgG {
   gen_prog_name_target : gname;
   gen_prog_name_source : gname;
-  gen_prog_inG_source :> gen_progPreNameG F C_s Σ gen_prog_name_source;
-  gen_prog_inG_target :> gen_progPreNameG F C_t Σ gen_prog_name_target;
+  gen_prog_inG_source :> gen_progGS_named F C_s Σ gen_prog_name_source;
+  gen_prog_inG_target :> gen_progGS_named F C_t Σ gen_prog_name_target;
 }.
 
 Global Arguments GenSimProgG F C_t C_s Σ {_ _} _ _ {_ _}.
@@ -27,7 +27,7 @@ Global Arguments gen_prog_name_source {F C_t C_s Σ _ _} _ : assert.
 Global Arguments gen_prog_name_target {F C_t C_s Σ _ _} _ : assert.
 
 Section definitions.
-  Context `{Countable F, gen_prog_name : gname, hG : !gen_progPreNameG F C Σ gen_prog_name }.
+  Context `{Countable F, gen_prog_name : gname, hG : !gen_progGS_named F C Σ gen_prog_name }.
 
   Definition gen_prog_interp (P : gmap F C) : iProp Σ :=
     ghost_map_auth gen_prog_name 1 P.
@@ -43,7 +43,7 @@ Local Notation "f @ K" := (hasfun f K)
   (at level 20, format "f  @  K") : bi_scope.
 
 Section gen_prog.
-  Context {F C} `{Countable L, gen_prog_name : gname, gen_progPreNameG F C Σ gen_prog_name}.
+  Context {F C} `{Countable L, gen_prog_name : gname, gen_progGS_named F C Σ gen_prog_name}.
   Implicit Types P Q : iProp Σ.
   Implicit Types p : gmap F C.
 
@@ -89,22 +89,22 @@ Section gen_prog.
   Qed.
 End gen_prog.
 
-Lemma gen_prog_init_names `{Countable F, !gen_progPreG F C Σ} p :
+Lemma gen_prog_init_names `{Countable F, !gen_progGpreS F C Σ} p :
   ⊢ |==> ∃ γp : gname,
-    let hG := GenProgPreNameG F C Σ γp in
+    let hG := GenProgGSNamed F C Σ γp in
     gen_prog_interp p ∗ ([∗ map] f ↦ K ∈ p, f @ K).
 Proof.
   iMod (ghost_map_alloc_empty (K:=F) (V:=C)) as (γp) "Hp".
   iExists γp.
-  iAssert (gen_prog_interp (hG:=GenProgPreNameG _ _ _ γp _ _ _) ∅) with "[Hp]" as "Hinterp";
+  iAssert (gen_prog_interp (hG:=GenProgGSNamed _ _ _ γp _ _ _) ∅) with "[Hp]" as "Hinterp";
     first by iFrame "Hp".
   iMod (gen_prog_alloc_big with "Hinterp") as "(Hinterp & $)".
   { apply map_disjoint_empty_r. }
   rewrite right_id_L. done.
 Qed.
 
-Lemma gen_prog_init `{Countable F, !gen_progPreG F C_t Σ, !gen_progPreG F C_s Σ} P_t P_s :
-  ⊢ |==> ∃ _ : gen_sim_progG F C_t C_s Σ,
+Lemma gen_prog_init `{Countable F, !gen_progGpreS F C_t Σ, !gen_progGpreS F C_s Σ} P_t P_s :
+  ⊢ |==> ∃ _ : gen_sim_progGS F C_t C_s Σ,
     (gen_prog_interp (hG:=gen_prog_inG_target) P_t ∗
     ([∗ map] f ↦ K ∈ P_t, hasfun (hG:=gen_prog_inG_target) f K)) ∗
     (gen_prog_interp (hG:=gen_prog_inG_source) P_s ∗
